sel4_artifacts/UxASSeL4/CMASI/MissionCommandUtils.h
@@ -1,30 +1,33 @@
 #ifndef __MISSIONCOMMANDUTILS_H__
 #define __MISSIONCOMMANDUTILS_H__
 #include <stdbool.h>
-#include "MissionCommand.h"
+/*#include "MissionCommand.h"*/
+#include "Waypoint.h"
 
 int lmcp_process_msg(uint8_t** inb, size_t size, lmcp_object **o);
 int lmcp_unpack(uint8_t** inb, size_t size, lmcp_object **o);
 
 
-struct MissionCommandExt_struct{
+/*struct MissionCommandExt_struct{
   MissionCommand missioncommand;
   Waypoint * waypoints;
   uint16_t waypointslen;
 
 };
 
-typedef struct MissionCommandExt_struct MissionCommandExt;
+typedef struct MissionCommandExt_struct MissionCommandExt; 
 
-void MCEInit(MissionCommandExt * mce, uint16_t waypoints);
-void MCWaypointSubSequence(const MissionCommand * omcp,
-                           const int64_t id,
-                           const uint16_t len,
-                            Waypoint * waypoints);
-bool GetMCWaypointSubSequence(const MissionCommand * omcp,
-                              const int64_t last_prefix_start_id,
-                              const int64_t ap_id,
-                              const uint16_t len,
-                              MissionCommandExt * wmcp);
-
+void MCEInit(MissionCommandExt * mce, uint16_t waypoints);*/
+Waypoint * FindWP(Waypoint * ws, uint16_t len, int64_t id);
+void MCWaypointSubSequence(  Waypoint * ws
+                           , uint16_t len_ws
+                           , int64_t id
+                           , uint16_t len_ws_win
+                             , Waypoint * ws_win /* out */);
+bool GetMCWaypointSubSequence( Waypoint * ws
+                             , uint16_t len_ws
+                             , int64_t last_start_id
+                             , int64_t approach_id
+                             , uint16_t len_ws_win
+                               , Waypoint * ws_win /* out */ );
 #endif /* __MISSIONCOMMANDUTILS_H__ */
