sel4_artifacts/UxASSeL4/verification/ImplToFunSpec.thy
@@ -2,288 +2,241 @@ theory ImplToFunSpec imports
 "LoadCode"
 "WaypointManagerFunSpec"
 begin
-
+  
+  
 definition nextwp_update where
 "nextwp_update w i \<equiv>   nextwaypoint_C_update (\<lambda> _. i) w"
 
-interpretation WaypointManager get_waypoint_number nextwaypoint_C nextwp_update
+interpretation WaypointManager number_C nextwaypoint_C nextwp_update
   apply unfold_locales
     apply (auto simp add: nextwp_update_def)
-  using Waypoint_struct_C_accupd_diff(131) get_waypoint_number_def nextwp_update_def apply presburger  
   done
-    
-    
-(* Lift waypoints from a mission command into a list with the same order. *)
+ 
+(* Lift waypoints list in memory into a list. *)
 fun lift_waypoints  where
-  "lift_waypoints s mcp 0 = []"
-| "lift_waypoints s mcp (Suc n) = lift_waypoints s mcp n @ [get_waypoint s mcp n]" 
+  "lift_waypoints s wsp 0 = []"
+| "lift_waypoints s wsp (Suc n) 
+  = lift_waypoints s wsp n @ [heap_Waypoint_struct_C s (wsp +\<^sub>p int n)]" 
 
 (* lift_waypoints maintains the size waypoints lifted. *)
-lemma lift_waypoints_length: "ws = lift_waypoints s mcp n \<Longrightarrow> length ws = n"
+lemma lift_waypoints_length: "ws = lift_waypoints s wsp n \<Longrightarrow> length ws = n"
   apply(induct n arbitrary: ws) by auto  
 
 (* One can use nth to get waypoint i indirectly through lift_waypoints. *)
 lemma lift_waypoints_to_get_waypoint: 
-  "ws = lift_waypoints s mcp n \<Longrightarrow> \<forall> k< n.  get_waypoint s mcp k = nth ws k"
-apply(induct n arbitrary: ws) by (auto simp add: less_Suc_eq lift_waypoints_length nth_append)
+  "ws = lift_waypoints s wsp n \<Longrightarrow> \<forall> k< n.  heap_Waypoint_struct_C s (wsp +\<^sub>p k) = nth ws k"
+  apply(induct n arbitrary: ws) 
+   apply auto
+    by (metis less_antisym lift_waypoints_length nth_append nth_append_length)
     
 lemma lift_waypoint_to_take:
-  "ws = lift_waypoints s mcp i \<Longrightarrow> j < i \<Longrightarrow> take j ws = lift_waypoints s mcp j"
+  "ws = lift_waypoints s wsp i \<Longrightarrow> j < i \<Longrightarrow> take j ws = lift_waypoints s wsp j"
 proof(induct j arbitrary: ws)
   case 0
   then show ?case by auto
 next
   case (Suc j)
-  then have "take j ws = lift_waypoints s mcp j" by auto
+  then have "take j ws = lift_waypoints s wsp j" by auto
   thus ?case using Suc
-    by (metis Suc_lessD lift_waypoints.simps(2) lift_waypoints_length lift_waypoints_to_get_waypoint 
-        take_Suc_conv_app_nth)
+    by (metis less_asym' lift_waypoints.simps(2) lift_waypoints_length 
+        lift_waypoints_to_get_waypoint not_less_eq take_Suc_conv_app_nth)
 qed
   
 lemma find_waypoint_extend_failure:
-  assumes a1:"None = find_waypoint (lift_waypoints s mcp (unat (j::32 word))) i"
-and a2:"number_C (get_waypoint s mcp (uint j)) \<noteq> i"
+assumes a1:"None = find_waypoint (lift_waypoints s wsp (unat (j::16 word))) i"
+and a2:"number_C (heap_Waypoint_struct_C s (wsp +\<^sub>p (uint j))) \<noteq> i"
 and a3:"j < k"
-shows "None = find_waypoint (lift_waypoints s mcp (unat (j + 1))) i"
+shows "None = find_waypoint (lift_waypoints s wsp (unat (j + 1))) i"
 proof -
-  have y1:"None = find_waypoint ( lift_waypoints s mcp (unat j) @ [get_waypoint s mcp (uint j)]) i" 
-    by (metis get_waypoint_number_def a1 a2 find_waypoint_none_extend)
-  then have y2:"None = find_waypoint (lift_waypoints s mcp (Suc (unat j))) i" by (simp add: uint_nat)
+  have y1:"None = find_waypoint ( lift_waypoints s wsp (unat j) 
+                  @ [heap_Waypoint_struct_C s (wsp +\<^sub>p (uint j))]) i" 
+    using a1 a2 find_waypoint_none_extend by blast
+  then have y2:"None = find_waypoint (lift_waypoints s wsp (Suc (unat j))) i"
+    by (simp add: uint_nat)
   then have y3:"(unat j) + 1 = unat (j + 1)" using a3 
     by (metis Suc_eq_plus1 add.commute less_is_non_zero_p1 unatSuc)
   thus ?thesis using Suc_eq_plus1 y2 by presburger
 qed
 
-lemma find_waypoint_failure_all_neq_number:"ws = lift_waypoints s mcp (unat (get_waypoints_length s mcp)) 
+lemma find_waypoint_failure_all_neq_number:
+"ws = lift_waypoints s wsp j 
 \<Longrightarrow> None = find_waypoint ws n
-\<Longrightarrow> \<forall>i<unat (get_waypoints_length s mcp). number_C (get_waypoint s mcp (int i)) \<noteq> n"
-  by (metis find_waypoint_failure_not_equal_all_elems 
-      get_waypoint_number_def lift_waypoints_length lift_waypoints_to_get_waypoint)
+\<Longrightarrow> \<forall>i< j. number_C (heap_Waypoint_struct_C s (wsp +\<^sub>p (int i))) \<noteq> n"
+  by (simp add: find_waypoint_failure_not_equal_all_elems lift_waypoints_length 
+      lift_waypoints_to_get_waypoint)
 
-lemma valid_mission_command[simp]:
-"is_valid_MissionCommand s mcp 
-\<Longrightarrow> j < get_waypoints_length s mcp
-\<Longrightarrow> is_valid_MissionCommand_struct_C s mcp 
-  \<and> is_valid_Waypoint_struct_C s (get_waypoint_ptr s mcp (uint j)) 
-  \<and> is_valid_Waypoint_struct_C'ptr s (get_waypoint_ptr_ptr s mcp (uint j)) 
-  \<and> is_valid_MissionCommand_struct_C s mcp"
-  apply(unfold is_valid_MissionCommand_def) by (metis uint_nat word_less_nat_alt)  
-  
-lemma findwp_success:
-"\<lbrace> \<lambda> (s::lifted_globals).
-  is_valid_MissionCommand s mcp
-  \<and> Some w = find_waypoint (lift_waypoints s mcp (unat (get_waypoints_length s mcp))) i
-  \<and> P s\<rbrace>
-   LoadCode.MissionCommandUtils.FindWP' mcp i
-\<lbrace> \<lambda> r s.   is_valid_MissionCommand s mcp
-  \<and> Some w = find_waypoint (lift_waypoints s mcp (unat (get_waypoints_length s mcp))) i \<and> P s \<and> heap_Waypoint_struct_C s r = w\<rbrace>!"
-  apply (unfold LoadCode.MissionCommandUtils.FindWP'_def)
-  apply (simp add: skipE_def)
-  apply(subst whileLoopE_add_inv
-        [where 
-          M = "\<lambda> (j,s). unat (get_waypoints_length s mcp - j)"
-          and I = 
-            "\<lambda> j s. P s 
-            \<and> is_valid_MissionCommand s mcp
-            \<and> Some w = find_waypoint (lift_waypoints s mcp (unat (get_waypoints_length s mcp))) i
-            \<and> None = find_waypoint (lift_waypoints s mcp (unat j)) i
-            \<and> j \<le> get_waypoints_length s mcp"
-        ])
-  apply wp
-    apply clarsimp
-    apply rule+
-     apply (metis find_waypoint_next_is_match lift_waypoints_length 
-      lift_waypoints_to_get_waypoint lift_waypoint_to_take uint_nat unat_mono)
-    apply (metis find_waypoint_extend_failure get_waypoint_number_def inc_le) 
-   apply force
-  apply wp
-  using find_waypoint_def is_valid_MissionCommand_def by auto
-  
-lemma findwp_failure:
-"\<lbrace> \<lambda> (s::lifted_globals).
-  P s
-  \<and> is_valid_MissionCommand s mcp
-  \<and> None = find_waypoint (lift_waypoints s mcp (unat (get_waypoints_length s mcp))) i \<rbrace>
-  LoadCode.MissionCommandUtils.FindWP' mcp i
-\<lbrace> \<lambda> r s. P s \<and> r = NULL \<rbrace>!"
-  apply (unfold LoadCode.MissionCommandUtils.FindWP'_def)
-  apply (simp add: skipE_def)
-  apply(subst whileLoopE_add_inv
-        [where 
-          M = "\<lambda> (j,s). unat (get_waypoints_length s mcp - j)"
-          and I = "\<lambda> j s. P s 
-                          \<and> is_valid_MissionCommand s mcp
-                          \<and> None 
-                            = find_waypoint 
-                                (lift_waypoints s mcp (unat (get_waypoints_length s mcp))) 
-                                i"
-        ])
- apply wp
-    apply clarsimp
-    apply (metis find_waypoint_failure_all_neq_number get_waypoint_number_def 
-                 uint_nat word_less_nat_alt)
-  apply simp
-  apply wp
-  using is_valid_MissionCommand_def by auto
-
-    
-lemma findwp_to_funspec:
-"\<lbrace> \<lambda> (s::lifted_globals).
-  is_valid_MissionCommand s mcp
-  \<and> P s \<rbrace>
-  LoadCode.MissionCommandUtils.FindWP' mcp i
-\<lbrace> \<lambda> r s. 
-  
-  r = NULL \<longrightarrow> None = find_waypoint (lift_waypoints s mcp (unat (get_waypoints_length s mcp))) i
-  \<and> r \<noteq> NULL 
-    \<longrightarrow> is_valid_Waypoint_struct_C s r 
-        \<and> Some (heap_Waypoint_struct_C s r) 
-          = find_waypoint (lift_waypoints s mcp (unat (get_waypoints_length s mcp))) i 
-  \<and> P s\<rbrace>!"
- apply (unfold LoadCode.MissionCommandUtils.FindWP'_def)
- apply (simp add: skipE_def)
- apply(subst whileLoopE_add_inv
-      [where 
-          M = "\<lambda> (j,s). unat (get_waypoints_length s mcp - j)"
-          and I = 
-            "\<lambda> j s. P s 
-             \<and> is_valid_MissionCommand s mcp
-             \<and> None = find_waypoint (lift_waypoints s mcp (unat j)) i
-             \<and> (get_waypoint_number (get_waypoint s mcp (uint j)) = i 
-                \<or> get_waypoint_number (get_waypoint s mcp (uint j)) \<noteq> i)
-             \<and> j \<le> get_waypoints_length s mcp"
-      ])
-  apply wp
-    apply clarsimp
-    apply (metis find_waypoint_extend_failure get_waypoint_number_def inc_le)
-    apply blast
-  apply wp
-  using find_waypoint_def is_valid_MissionCommand_def by auto    
-
-lemma max_word16[simp]:"(max_word::16 word) = 65535"    
-  apply(unfold max_word_def) by auto
-
-lemma word16_leq_max_word16:"uint (a::16 word) \<le> 65535"
-  using word.uint[of a] by auto
-    
-lemma word16_leq_max_word32:"uint (a::16 word) \<le> 2147483648"
-  using word.uint[of a] by auto
-    
-theorem validNF_bind_return:"\<lbrace> A \<rbrace> g f \<lbrace>B\<rbrace>! \<Longrightarrow> \<lbrace>A\<rbrace> (return f) >>= g \<lbrace>B\<rbrace>!"   
-  apply (rule validNF_bind[ where B="\<lambda> r s. A s \<and> r = f"])
-   apply (simp add: triple_judgement_def validNF_is_triple)
-    by (smt hoare_return_simp no_fail_pre no_fail_return validNF)
-
-theorem validNF_bind_gets:"\<forall> r. \<lbrace> \<lambda> s. A s \<and> r = f s \<rbrace> g r \<lbrace>B\<rbrace>! \<Longrightarrow> \<lbrace>A\<rbrace> do x \<leftarrow> gets f; g x od\<lbrace>B\<rbrace>!"   
-  apply (rule validNF_bind[ where B="\<lambda> r s. A s \<and> r = f s"])
-   apply simp
-  by (simp add: hoare_gets validNF)
-
-theorem validNF_ignbind_modify:"\<forall> s. A (f s) = A s \<Longrightarrow> \<forall> r. \<lbrace> \<lambda> s. A (f s) \<rbrace> g \<lbrace>B\<rbrace>! \<Longrightarrow> \<lbrace>A\<rbrace> do x \<leftarrow> modify f; g od\<lbrace>B\<rbrace>!"   
-  apply (rule validNF_bind[ where B="\<lambda> r s. A (f s)"])
-   apply simp
-    by (metis hoare_modifyE_var no_fail_def no_fail_modify validNF)
       
-      
-lemma validNF_nobind_guard:" \<forall> s. P s \<longrightarrow> Q s \<Longrightarrow> \<lbrace> P \<rbrace> S \<lbrace> R \<rbrace>! \<Longrightarrow> \<lbrace> P \<rbrace> do guard Q; S od \<lbrace> R \<rbrace>!"
-  apply wp by (simp add: guard_def validNF_alt_def)
-    
-lemma validNF_bind_guard:" \<forall> s. P s \<longrightarrow> Q s \<Longrightarrow> \<lbrace> P \<rbrace> S  \<lbrace> R \<rbrace>! \<Longrightarrow> \<lbrace> P \<rbrace> do x \<leftarrow> guard Q; S od \<lbrace> R \<rbrace>!"
-  apply wp by (simp add: guard_def validNF_alt_def)
-    
-lemma validNF_bind_FindWP:
-"\<forall> r. \<lbrace>\<lambda> s. is_valid_MissionCommand s mcp \<and> Some w = find_waypoint (lift_waypoints s mcp (unat (get_waypoints_length s mcp))) i \<and> P s \<and> heap_Waypoint_struct_C s r = w\<rbrace> S r \<lbrace> R \<rbrace>! 
-\<Longrightarrow> \<lbrace> \<lambda> s. is_valid_MissionCommand s mcp \<and> Some w = find_waypoint (lift_waypoints s mcp (unat (get_waypoints_length s mcp))) i \<and> P s\<rbrace> do x  \<leftarrow> LoadCode.MissionCommandUtils.FindWP' mcp i; S x od \<lbrace> R \<rbrace>!"
-  apply (rule validNF_bind[where B="\<lambda> r s. is_valid_MissionCommand s mcp \<and> Some w = find_waypoint (lift_waypoints s mcp (unat (get_waypoints_length s mcp))) i \<and> P s \<and> heap_Waypoint_struct_C s r = w"])
-   apply auto
-  by (rule findwp_success)
-  
-lemma test:"(\<forall> s. P s \<longrightarrow> (\<exists> w. find_waypoint (lift_waypoints s mcp (unat (get_waypoints_length s mcp))) i = Some w))
-\<Longrightarrow> (\<forall> s. P s \<longrightarrow> (\<forall> r. (heap_Waypoint_struct_C s r) = w \<and> Q r s)) \<Longrightarrow>
-\<lbrace>  P \<rbrace> MissionCommandUtils.FindWP' mcp i \<lbrace> Q \<rbrace>!"
-  sorry
-        
-lemma validNF_bind_rev: "\<lbrace>A\<rbrace> f \<lbrace>B\<rbrace>! \<Longrightarrow> (\<And>x. \<lbrace>B x\<rbrace> g x \<lbrace>C\<rbrace>!) \<Longrightarrow> \<lbrace>A\<rbrace> f >>= g \<lbrace>C\<rbrace>!"
-  by (rule validNF_bind)
-
-(* Structures must be packed! *)
-lemma ac_bug_nextwaypoint_update[simp]:"P s[wsp +\<^sub>p j \<rightarrow>nextwaypoint :=  w] = P s[wsp +\<^sub>p j := LoadCode.Waypoint_struct_C.nextwaypoint_C_update (\<lambda> _. w) (heap_Waypoint_struct_C s (wsp +\<^sub>p j))]"
-  sorry
-    
-lemma ac_bug_number_fetch[simp]:"s[wsp +\<^sub>p (uint n - 1)]\<rightarrow>number = number_C (heap_Waypoint_struct_C s (wsp +\<^sub>p (uint n - 1)))"
-  sorry
- 
-(*    
-lemma aux:
-  assumes asm1:"0 < n"
-  and asm2:"\<forall>s v j. j < unat (n::word16) \<longrightarrow> P s[(wsp::Waypoint_struct_C ptr) +\<^sub>p int j := v] = P s"
-  and asm3:"P s"
-  shows "P (LoadCode.MissionCommandUtils.update_Waypoint_struct s (wsp +\<^sub>p (uint n - 1)) w)"
+lemma lift_waypoints_next_success:
+assumes a1:"ws = (lift_waypoints s wsp len)"
+and a2:"Some w = find_waypoint ws i"
+and a3:"None = find_waypoint (take j ws)  i"
+and a4:"j < len"
+and a5:"i = s[wsp +\<^sub>p j]\<rightarrow>number"
+shows "Some s[wsp +\<^sub>p j] = find_waypoint ws s[wsp +\<^sub>p j]\<rightarrow>number"
 proof -
-  have y1:"unat (n - 1) < unat n" using asm1 measure_unat by force
-  then have y2:"P s[wsp +\<^sub>p int (unat n - 1) := w]" using asm3 asm1 asm2 unat_minus_one word_neq_0_conv by fastforce
-  then have "int (unat n - 1) = uint n - 1" 
-    by (metis (no_types, hide_lams) cancel_comm_monoid_add_class.diff_cancel nat_less_cases' not_less of_nat_1 of_nat_diff of_nat_less_iff semiring_1_class.of_nat_0 uint_nat uint_nonnegative y1)      
-  thus ?thesis using y2 by auto
+  have y1:"i = number_C (ws !  j)" 
+    by (metis MissionCommandUtils.get_Waypoint_struct_number_def a1 a4 a5 lift_waypoints_to_get_waypoint uint_nat word_less_nat_alt)
+  then have y2:"Some w = find_waypoint ws (number_C (ws ! j))" using a2 y1 by auto
+  then have y3:"j < length ws" using a2 a3 not_less by fastforce
+  then have "ws ! j = w" using find_waypoint_next_is_match[OF y2 _ y3] a3 y1 by auto
+  thus ?thesis by (metis a1 a2 a4 a5 lift_waypoints_to_get_waypoint)
 qed
-*)  
-lemma nextwp_update_rewrite[simp]:"nextwaypoint_C_update (\<lambda>_. get_waypoint_number s[wsp +\<^sub>p j]) s[wsp +\<^sub>p j] 
-              = nextwp_update s[wsp +\<^sub>p j] (get_waypoint_number s[wsp +\<^sub>p j])"
-  sorry
-  
-lemma aux2:"              0 < n \<Longrightarrow>
-              is_valid_MissionCommand s mcp \<Longrightarrow>
-              Some win = waypoints_window (lift_waypoints s mcp (unat (get_waypoints_length s mcp))) i (unat n) 
-\<Longrightarrow> nextwp_update sa[wsp +\<^sub>p (uint n - 1)] (get_waypoint_number sa[wsp +\<^sub>p (uint n - 1)]) = win ! j"    
-  sorry
+     
+lemma lift_waypoints_take_id:"(take len (lift_waypoints s wsp len)) = (lift_waypoints s wsp len)"
+  apply(induct len)
+   apply auto
+    by (simp add: lift_waypoints_length)
 
-lemma aux3:" 0 < (n::word16) \<Longrightarrow> INT_MIN < uint n"
-  sorry
+lemma findwp_success_supp1:
+"
+Some w = find_waypoint (lift_waypoints s wsp len) i 
+\<Longrightarrow>
+None = find_waypoint (take j (lift_waypoints s wsp len)) i 
+\<Longrightarrow>
+j < len 
+\<Longrightarrow> 
+s[wsp +\<^sub>p int j]\<rightarrow>number \<noteq> i 
+\<Longrightarrow> None = find_waypoint (take (Suc j) (lift_waypoints s wsp len)) i"
+  by (metis MissionCommandUtils.get_Waypoint_struct_number_def find_waypoint_none_extend 
+      lift_waypoints_length lift_waypoints_to_get_waypoint take_Suc_conv_app_nth)
+      
+lemma findwp_success_aux:
+"
+len \<le> USHORT_MAX 
+\<Longrightarrow> 
+\<lbrace> \<lambda> (s::lifted_globals).
+  are_valid_Waypoints s wsp len
+  \<and> (\<exists> w. Some w = find_waypoint (lift_waypoints s wsp len) i)
+  \<and> P s\<rbrace>
+   LoadCode.MissionCommandUtils.FindWP' wsp len i
+\<lbrace> \<lambda> r s. are_valid_Waypoints s wsp len
+  \<and> Some (heap_Waypoint_struct_C s r) = find_waypoint (lift_waypoints s wsp len) i 
+  \<and> is_valid_Waypoint_struct_C s r 
+  \<and> P s \<rbrace>!"
+  apply (unfold LoadCode.MissionCommandUtils.FindWP'_def)
+  apply (unfold skipE_def)
+  apply wp
+  apply(subst whileLoopE_add_inv
+        [where 
+          M = "\<lambda> (j,s). len - j"
+          and I = 
+            "\<lambda> j s.
+            are_valid_Waypoints s wsp len 
+            \<and> (\<exists> w. Some w = find_waypoint (lift_waypoints s wsp len) i)
+            \<and> None = find_waypoint (take j (lift_waypoints s wsp len)) i
+            \<and> P s
+            \<and> j \<le> len"
+        ])
+  apply wp
+    apply clarsimp  
+    using lift_waypoints_next_success findwp_success_supp1 findwp_success_supp1 max_short_fix apply fastforce
+   by (clarsimp, simp add: lift_waypoints_take_id find_waypoint_def)+    
+ 
+lemma findwp_success[wp]: 
+" 
+len \<le> USHORT_MAX 
+\<Longrightarrow> 
+(\<forall> s. P s \<longrightarrow>  (are_valid_Waypoints s wsp len \<and> (\<exists> w. Some w = find_waypoint (lift_waypoints s wsp len) i))) 
+\<Longrightarrow>
+\<forall> r. 
+\<lbrace>\<lambda> s::lifted_globals. 
+  are_valid_Waypoints s wsp len 
+  \<and> Some (heap_Waypoint_struct_C s r) = find_waypoint (lift_waypoints s wsp len) i 
+  \<and> is_valid_Waypoint_struct_C s r \<and> P s\<rbrace> 
+g r 
+\<lbrace> Q \<rbrace>!
+\<Longrightarrow>
+\<lbrace> P \<rbrace> 
+do x \<leftarrow> MissionCommandUtils.FindWP' wsp len i; 
+        g x 
+od 
+\<lbrace> Q \<rbrace>!"
+  apply (rule validNF_bind[where B="\<lambda> r s. are_valid_Waypoints s wsp len \<and> Some (heap_Waypoint_struct_C s r) = find_waypoint (lift_waypoints s wsp len) i \<and> is_valid_Waypoint_struct_C s r \<and> P s"])
+   apply simp
+  apply (rule validNF_weaken_pre[where Q="\<lambda> s. are_valid_Waypoints s wsp len \<and> (\<exists>w. Some w = find_waypoint (lift_waypoints s wsp len) i) \<and> P s"])
+    apply (rule findwp_success_aux)
+  by auto
 
-lemma aux4:"uint (n::word16) \<le> 2147483648"
-  sorry
+lemma forward_validNF_guard_nobind[wp]:"\<lbrace> \<lambda> s. P s \<and> f s\<rbrace> g \<lbrace> Q \<rbrace>! \<Longrightarrow> (\<forall> s. P s \<longrightarrow> f s) \<Longrightarrow> \<lbrace> P \<rbrace> do guard f; g od \<lbrace> Q \<rbrace>!"
+  apply (rule validNF_bind[where B = "\<lambda> r s. P s \<and> f s"])
+   apply simp
+  apply wp
+  by auto
+   
+lemma forward_validNF_guard_bind:"\<lbrace> \<lambda> s. P s \<and> f s\<rbrace> g \<lbrace> Q \<rbrace>! \<Longrightarrow> (\<forall> s. P s \<longrightarrow> f s) \<Longrightarrow> \<lbrace> P \<rbrace> do  x \<leftarrow> guard f; g od \<lbrace> Q \<rbrace>!"
+  apply (rule validNF_bind[where B = "\<lambda> r s. P s \<and> f s"])
+   apply simp
+  apply wp
+  by auto    
+    
+lemma forward_validNF_modify[wp]:"\<lbrace> P \<rbrace> g \<lbrace> Q \<rbrace>! \<Longrightarrow> (\<forall> s. P s \<longrightarrow> P (f s)) \<Longrightarrow> \<lbrace> P \<rbrace> do x \<leftarrow> modify f; g od \<lbrace> Q \<rbrace>!"
+  apply wp
+  by (simp add: hoare_modifyE_var no_fail_def snd_modify validNF_def)    
+    
+lemma forward_validNF_whileloop_inv:" \<lbrace> P \<rbrace> whileLoop_inv c s v i m\<lbrace> \<lambda> r s. P s \<and> i r s \<and> \<not>(c r s) \<rbrace>! \<Longrightarrow> \<forall> r. \<lbrace> \<lambda> s. P s \<and> i r s \<and> \<not>(c r s) \<rbrace> g r \<lbrace> Q \<rbrace>!  \<Longrightarrow> \<lbrace> P \<rbrace> do x \<leftarrow> whileLoop_inv c s v i m; g x od \<lbrace> Q \<rbrace>!"
+  apply (rule validNF_bind[where B = " \<lambda> r s. P s \<and> i r s \<and> \<not>(c r s)"])
+    by auto
 
-lemma aux5:"-2147483648 < uint (n::word16) "
+lemma forward_validNF_gets[wp]:"\<forall> x. \<lbrace> \<lambda> s. P s \<and> x = f s \<rbrace> g x \<lbrace> Q \<rbrace>! \<Longrightarrow> \<lbrace> P \<rbrace> do x \<leftarrow> gets f; g x od \<lbrace> Q \<rbrace>!"
+  apply (rule validNF_bind[where B="\<lambda> x s. P s \<and> x = f s"])
+   apply blast
+  apply wp
+    by auto
+   
+lemma are_valid_waypoints_noninter1:" ws1p +\<^sub>p len = ws2p \<Longrightarrow>  are_valid_Waypoints s ws1p len \<Longrightarrow> are_valid_Waypoints s[(ws2p::Waypoint_struct_C ptr) +\<^sub>p (k::nat) := v] ws1p len"
+  apply (unfold are_valid_Waypoints_def) by auto
+    
+lemma are_valid_waypoints_noninter2:"ws1p +\<^sub>p len = ws2p \<Longrightarrow>  are_valid_Waypoints s[((ws2p::Waypoint_struct_C ptr) +\<^sub>p (k::nat))\<rightarrow>nextwaypoint := v] ws1p len =  are_valid_Waypoints s ws1p len"
+     apply (unfold are_valid_Waypoints_def) by auto
+    
+lemma lift_waypoints_noninter1:"ws1p +\<^sub>p len = ws2p \<Longrightarrow>  lift_waypoints s[(ws2p::Waypoint_struct_C ptr) +\<^sub>p (k::nat) := v] ws1p len = lift_waypoints s ws1p len"
   sorry
     
-lemma aux6:"0 < n \<Longrightarrow> \<forall>k<unat n. is_valid_Waypoint_struct_C sa (wsp +\<^sub>p int k) \<Longrightarrow> is_valid_Waypoint_struct_C sa (wsp +\<^sub>p (uint n - 1))"
-  by (metis One_nat_def Suc_diff_1 le_less lessI neq0_conv of_nat_1 of_nat_diff uint_nat unat_0 word_less_nat_alt zero_less_diff)
+lemma lift_waypoints_noninter2:"ws1p +\<^sub>p len = ws2p \<Longrightarrow>  lift_waypoints s[((ws2p::Waypoint_struct_C ptr) +\<^sub>p k)\<rightarrow>nextwaypoint := v] ws1p len =  lift_waypoints s ws1p len"
+  sorry
     
+lemma update_with_valid[simp]:"are_valid_Waypoints s p l \<Longrightarrow>
+           is_valid_Waypoint_struct_C s r \<Longrightarrow>
+           are_valid_Waypoints s[p := s[r]] p l"
+  apply (unfold are_valid_Waypoints_def)
+  by auto
+      
 lemma MCWaypointSubSequence_to_funspec:
-"(\<forall> s v j. j < unat n \<longrightarrow> P (LoadCode.MissionCommandUtils.update_Waypoint_struct s (wsp +\<^sub>p j) v) = P s) \<Longrightarrow>
-  \<lbrace>\<lambda> (s::lifted_globals). 
-  n > 0
-  \<and> is_valid_MissionCommand s mcp
-  \<and> ws = lift_waypoints s mcp (unat (get_waypoints_length s mcp))
-  \<and> Some win = waypoints_window ws i (unat n)
-  \<and> is_valid_Waypoint_struct_C s wsp
-  \<and> (\<forall> j. j < unat n \<longrightarrow> is_valid_Waypoint_struct_C s (wsp +\<^sub>p j))
-  \<and> P s \<rbrace>
-  LoadCode.MissionCommandUtils.MCWaypointSubSequence' mcp i n wsp 
+"len_ws \<le> USHORT_MAX
+\<Longrightarrow> wsp +\<^sub>p len_ws = ws_winp
+\<Longrightarrow> waypoints_wf ws
+\<Longrightarrow> Some win = waypoints_window ws i  len_ws_win
+\<Longrightarrow> len_ws_win \<le> len_ws 
+\<Longrightarrow> 0<len_ws
+\<Longrightarrow> 0<len_ws_win
+\<Longrightarrow> \<lbrace>\<lambda> (s::lifted_globals). 
+  are_valid_Waypoints s ws_winp len_ws_win
+  \<and>  are_valid_Waypoints s wsp len_ws
+  \<and> ws = lift_waypoints s wsp len_ws\<rbrace>
+  LoadCode.MissionCommandUtils.MCWaypointSubSequence' wsp len_ws i len_ws_win ws_winp
 \<lbrace> \<lambda> r s. 
-  P s 
-  \<and> (\<forall> j. j < unat n \<longrightarrow> heap_Waypoint_struct_C s (wsp +\<^sub>p j) = win ! j) \<rbrace>!"
-  apply (rule validNF_assume_pre)
+ (\<forall> j. j <  len_ws_win \<longrightarrow> heap_Waypoint_struct_C s (ws_winp +\<^sub>p j) = win ! j) \<rbrace>!"
   apply (unfold LoadCode.MissionCommandUtils.MCWaypointSubSequence'_def)
-  apply (subst whileLoop_add_inv[
-        where I="\<lambda>(j, idit) s. 
-  j \<le> n
-  \<and> is_valid_MissionCommand s mcp
-  \<and> (\<exists> win'. Some win' = waypoints_window ws i (unat j) \<and> prefix win' win)
-  \<and> is_valid_Waypoint_struct_C s wsp
-  \<and> (\<forall> k. k < unat j \<longrightarrow> is_valid_Waypoint_struct_C s (wsp +\<^sub>p k))
-  \<and> P s" 
-          and M="\<lambda>((i, idit),s).  unat n - unat i"],clarsimp)
-
-      apply (rule validNF_bind[where B="\<lambda> (j,idit) s. P s 
-  \<and> j = n
-  \<and> is_valid_Waypoint_struct_C s wsp
-  \<and> (\<forall> k. k < unat n \<longrightarrow> is_valid_Waypoint_struct_C s (wsp +\<^sub>p k))
-  \<and> (\<forall> j. j < unat n \<longrightarrow> heap_Waypoint_struct_C s (wsp +\<^sub>p j) = win ! j)"])
-   apply wp
-   apply (simp add: Product_Type.prod.case_eq_if)
-   sorry
-    
-  (* Trying to work forward. *)
+      apply(subst whileLoop_add_inv
+        [where 
+          M = "\<lambda> ((j,nid),s). len_ws_win - j"
+          and I = 
+            "\<lambda> (j,nid) s.
+  are_valid_Waypoints s ws_winp len_ws_win
+  \<and>  are_valid_Waypoints s wsp len_ws
+  \<and> ws = lift_waypoints s wsp len_ws
+            \<and> j < len_ws_win
+\<and> (j = 0 \<longrightarrow> nid = sint i)
+\<and> (0 < j \<longrightarrow> nid = sint (nextwaypoint_C (win ! (j - 1))))
+\<and>  (\<forall> k. k < j \<longrightarrow> heap_Waypoint_struct_C s (ws_winp +\<^sub>p k) = win ! k)
+"
+        ])
+  apply clarsimp
+     apply (rule forward_validNF_whileloop_inv)
+    apply (wp_once, clarsimp)
+     apply(rule forward_validNF_guard_nobind forward_validNF_gets forward_validNF_guard_bind forward_validNF_modify findwp_success | clarsimp)+
+  defer
+    defer
+      apply (wp | clarsimp )+ 
     
 end
